Adding ConnectNodes. Reasoning about validity and loops.

digraph.dfy
@@ -35,14 +35,197 @@ module Digraph {
         (forall i: nat :: i < |p.v|-1 ==> g.IsConnected(p.v[i], p.v[i+1]))
     }
 
-    ghost predicate {:opaque} PathLoop(p: Path)
+    predicate PathLoop(p: Path)
     {
-        (exists i: nat, j: nat :: i < |p.v| && j < |p.v| && i != j ==> p.v[i] == p.v[j])
+        |p.v| > 1 && p.v[0] == p.v[|p.v|-1]
     }
 
-    ghost predicate {:opaque} DigraphLoop(g: Digraph)
+    predicate PathNoRepeats(p: Path)
     {
-        exists p: Path :: PathValid(g, p) && PathLoop(p)
+        forall i: nat, j: nat :: i < |p.v| && j < |p.v| && i != j ==> p.v[i] != p.v[j]
+    }
+
+    predicate PathSimpleLoop(p: Path)
+    {
+        PathLoop(p) && PathNoRepeats(Path(p.v[1..|p.v|]))
+    }
+
+    function PathStart(p: Path): Node
+        requires |p.v| > 0
+    {
+        p.v[0]
+    }
+
+    function PathEnd(p: Path): Node
+        requires |p.v| > 0
+    {
+        p.v[|p.v|-1]
+    }
+
+    function PathRemoveLoops(p: Path): (r: Path)
+        requires |p.v| > 0
+    {
+        PathRemoveLoopsInternal(p, |p.v|-1)
+    }
+
+    function PathFindIndex(p: Path, n: Node): (r: nat)
+        requires n in p.v
+        ensures r < |p.v|
+        ensures p.v[r] == n
+    {
+        PathFindIndexInternal(p, n, 0)
+    }
+
+    function PathFindIndexInternal(p: Path, n: Node, index: nat): (r: nat)
+        requires index < |p.v|
+        requires n in p.v[index..|p.v|]
+        ensures r < |p.v|
+        ensures p.v[r] == n
+        decreases |p.v| - index
+    {
+        if p.v[index] == n then
+            index
+        else
+            PathFindIndexInternal(p, n, index+1)
+    }
+
+    function PathSegment(p: Path, start: nat, stop: nat): (r: Path)
+        requires start < |p.v|
+        requires stop <= |p.v|
+        requires start < stop
+        ensures |r.v| > 0
+    {
+        Path(p.v[start..stop])
+    }
+
+    lemma PathSegmentValid(g: Digraph, p: Path, start: nat, stop: nat)
+        requires start < |p.v|
+        requires stop <= |p.v|
+        requires start < stop
+        requires PathValid(g, p)
+        ensures 
+            var r := PathSegment(p, start, stop);
+            PathValid(g, r)
+    {
+        reveal PathValid();
+    }
+
+    function PathRemoveLoopsInternal(p: Path, index: nat): (r: Path)
+        requires index < |p.v|
+        decreases index
+    {
+        if index == 0 then
+            Path([p.v[0]])
+        else 
+            var earlier_path := PathRemoveLoopsInternal(p, index-1);
+            var n := p.v[index];
+            if n in earlier_path.v then
+                var loc := PathFindIndex(earlier_path, n);
+                Path(earlier_path.v[0..loc+1])
+            else
+                Path(earlier_path.v + [n])
+    }
+
+    lemma RemoveLoopsFromToSame(g: Digraph, p: Path)
+        requires |p.v| > 1
+        requires p.v[0] != p.v[|p.v|-1]
+        requires PathValid(g, p)
+        ensures
+            var a := p.v[0];
+            var b := p.v[|p.v|-1];
+            var q := PathRemoveLoops(p);
+            ShortPathFromTo(g, q, a, b)
+    {
+        RemoveLoopsFromToSameInternal(g, p, |p.v|-1);
+    }
+
+    lemma RemoveLoopsFromToSameInternal(g: Digraph, p: Path, index: nat)
+        requires index < |p.v|
+        requires |p.v| > 1
+        requires p.v[0] != p.v[|p.v|-1]
+        requires PathValid(g, p)
+        ensures
+            var a := p.v[0];
+            var b := p.v[index];
+            var q := PathRemoveLoopsInternal(p, index);
+            ShortPathFromTo(g, q, a, b)
+    {
+        var a := p.v[0];
+        var b := p.v[index];
+        var q := PathRemoveLoopsInternal(p, index);
+        if index == 0 {
+            assert q == Path([a]);
+            reveal PathValid();
+            assert ShortPathFromTo(g, q, a, b);
+        } else {
+            var earlier_path := PathRemoveLoopsInternal(p, index-1);
+            RemoveLoopsFromToSameInternal(g, p, index-1);
+            var n := p.v[index];
+            if n in earlier_path.v {
+                var loc := PathFindIndex(earlier_path, n);
+                assert q == Path(earlier_path.v[0..loc+1]);
+            } else {
+                assert q == Path(earlier_path.v + [n]);
+            }
+            reveal PathValid();
+            assert PathValid(g, earlier_path);
+            assert PathValid(g, q);
+            assert ShortPathFromTo(g, q, a, b);
+        }
+    }
+
+    lemma RemoveLoopsNoRepeats(p: Path)
+        ensures
+            var q := PathRemoveLoopsInternal(p, index);
+            PathNoRepeats(q)
+    {
+        RemoveLoopsNoRepeatsInternal(p, 0);
+    }
+
+    lemma RemoveLoopsNoRepeatsInternal(p: Path, index: nat)
+        requires index < |p.v|
+        ensures
+            var q := PathRemoveLoopsInternal(p, index);
+            PathNoRepeats(q)
+    {
+        var q := PathRemoveLoopsInternal(p, index);
+        if index == 0 {
+            var q := Path([p.v[0]]);
+            assert |q.v| == 1;
+            assert PathNoRepeats(q);
+        } else { 
+            var earlier_path := PathRemoveLoopsInternal(p, index-1);
+            var n := p.v[index];
+            if n in earlier_path.v {
+                var loc := PathFindIndex(earlier_path, n);
+                var q := Path(earlier_path.v[0..loc+1]);
+                assert PathNoRepeats(q);
+            } else {
+                var q := Path(earlier_path.v + [n]);
+                assert PathNoRepeats(q);
+            }
+        }
+    }
+
+    ghost predicate PathExists(g: Digraph, a: Node, b: Node)
+    {
+        exists p: Path :: PathFromTo(g, p, a, b)
+    }
+
+    predicate PathFromTo(g: Digraph, p: Path, a: Node, b: Node)
+    {
+        PathValid(g, p) && |p.v| > 1 && (p.v[0] == a) && (p.v[|p.v|-1] == b)
+    }
+
+    predicate SimplePathFromTo(g: Digraph, p: Path, a: Node, b: Node)
+    {
+        PathValid(g, p) && |p.v| > 1 && (p.v[0] == a) && (p.v[|p.v|-1] == b) &&
+        PathNoRepeats(Path(p.v[0..|p.v|-2]))
+    }
+
+    predicate ShortPathFromTo(g: Digraph, p: Path, a: Node, b: Node)
+    {
+        PathValid(g, p) && |p.v| > 0 && (p.v[0] == a) && (p.v[|p.v|-1] == b)
     }
 
     function PathIndex(p: Path, n: Node): (r: nat)
@@ -57,6 +240,41 @@ module Digraph {
         else
             PathIndex(Path(p.v[1..|p.v|]), n) + 1
     }
+
+    ghost predicate {:opaque} DigraphLoop(g: Digraph)
+    {
+        exists p: Path :: PathValid(g, p) && PathLoop(p)
+    }
+
+    ghost predicate {:opaque} DigraphLoop2(g: Digraph)
+    {
+        exists n: Node :: PathExists(g, n, n)
+    }
+
+    lemma DigraphLoopEquiv(g: Digraph)
+        ensures DigraphLoop(g) == DigraphLoop2(g)
+    {
+        reveal DigraphLoop();
+        reveal DigraphLoop2();
+        if DigraphLoop(g) {
+            var p :| PathValid(g, p) && PathLoop(p);
+            assert PathFromTo(g, p, p.v[0], p.v[0]);
+            assert PathExists(g, p.v[0], p.v[0]);
+        }
+    }
+
+    ghost function GetLoopPath(g: Digraph): (r: Path)
+        requires DigraphLoop(g)
+    {
+        reveal DigraphLoop();
+        DigraphLoopEquiv(g);
+        assert DigraphLoop2(g);
+        reveal DigraphLoop2();
+        var n :| PathExists(g, n, n);
+        var p :| PathValid(g, p) && |p.v| > 1 && p.v[0] == n && p.v[|p.v|-1] == n;
+        p
+    }
+
     
     // Adding nodes
 
@@ -68,6 +286,16 @@ module Digraph {
             g.IsConnected,
             if n >= g.NodeBound then n else g.NodeBound
         )
+    }
+
+    lemma AddNodeDigraphValid(g: Digraph, n: Node)
+        requires DigraphValid(g)
+        requires !g.IsNode(n)
+        ensures
+            var r := AddNode(g, n);
+            DigraphValid(r)
+    {
+        reveal DigraphValid();
     }
     
     // There is only one path that becomes valid when we add a node.
@@ -104,10 +332,6 @@ module Digraph {
         }
     }
 
-    lemma AddNodePathLoopConserved(g: Digraph, n: Node, p: Path)
-        requires !g.IsNode(n)
-    {
-    }
     /*
     When we add a node to a graph, that cannot introduce any loops.
     */
@@ -119,32 +343,23 @@ module Digraph {
             DigraphLoop(g) == DigraphLoop(r)
     {
         var r := AddNode(g, n);
-        // All the paths in the two graphs are the same except for one additional one in
-        // r which is [n]
         reveal PathValid();
-        forall p: Path {
-            if p == Path([n]) {
-                assert !g.IsNode(n);
-                NotNodePathInvalid(g, n, Path([n]));
-                assert !PathValid(g, p);
-                assert PathValid(r, p);
-                reveal PathLoop();
-                assert !PathLoop(p);
-            } else if PathValid(r, p) {
-                AddNodePathValid(g, n, p);
-                assert PathValid(g, p) || p == Path([n]);
-                assert PathValid(g, p);
-            } else {
-                assert !PathValid(g, p);
-            }
+        reveal DigraphLoop();
+        if DigraphLoop(g) {
+            var p := GetLoopPath(g);
+            assert PathValid(r, p);
+            assert DigraphLoop(r);
         }
-    }
-
-    lemma LengthOneNoLoop(p: Path)
-        requires |p| == 1
-        ensures NoLoop(p)
-    {
-        reveal NoLoop();
+        if DigraphLoop(r) {
+            var p :| PathValid(r, p) && PathLoop(p);
+            AddNodePathValid(g, n, p);
+            assert PathValid(g, p) || p == Path([n]);
+            if p == Path([n]) {
+                assert !PathLoop(p);
+            }
+            assert PathValid(g, p);
+            assert DigraphLoop(g);
+        }
     }
     
 
@@ -154,5 +369,197 @@ module Digraph {
         ensures !PathValid(g, p)
     {
         reveal PathValid();
+    }
+
+    // Connecting two nodes
+
+    function ConnectNodes(g: Digraph, n: Node, m: Node): (r: Digraph)
+        requires g.IsNode(n)
+        requires g.IsNode(m)
+        requires n != m
+        requires !g.IsConnected(n, m)
+    {
+        Digraph(
+            g.IsNode,
+            (a, b) => ((a==n) && (b==m)) || g.IsConnected(a, b),
+            g.NodeBound
+        )
+    }
+
+    lemma ConnectNodesDigraphValid(g: Digraph, n: Node, m: Node)
+        requires g.IsNode(n)
+        requires g.IsNode(m)
+        requires n != m
+        requires !g.IsConnected(n, m)
+        requires DigraphValid(g)
+        ensures
+            var r := ConnectNodes(g, n, m);
+            DigraphValid(r)
+    {
+        reveal DigraphValid();
+    }
+
+    lemma ConnectNodesPathStillValid(g: Digraph, n: Node, m: Node, p: Path)
+        requires g.IsNode(n) && g.IsNode(m) && n != m && !g.IsConnected(n, m)
+        requires PathValid(g, p)
+        ensures
+            var r := ConnectNodes(g, n, m);
+            PathValid(r, p)
+    {
+        reveal PathValid(); 
+    }
+
+    lemma ConnectNodesPathExists(g: Digraph, n: Node, m: Node)
+        requires g.IsNode(n) && g.IsNode(m) && n != m && !g.IsConnected(n, m)
+        ensures
+            var r := ConnectNodes(g, n, m);
+            PathExists(r, n, m)
+    {
+        var p := Path([n, m]);
+        var r := ConnectNodes(g, n, m);
+        assert r.IsConnected(n, m);
+        reveal PathValid();
+        assert PathFromTo(r, p, n, m);
+    }
+
+    lemma PathExistsAdd(g: Digraph, a: Node, b: Node, c: Node)
+        requires PathExists(g, a, b)
+        requires PathExists(g, b, c)
+        ensures PathExists(g, a, c)
+    {
+        var p :| PathFromTo(g, p, a, b);
+        var q :| PathFromTo(g, q, b, c);
+        assert |q.v| > 1;
+        var pq := Path(p.v[0..|p.v|] + q.v[1..|q.v|]);
+        reveal PathValid();
+        assert PathValid(g, pq);
+        assert PathFromTo(g, pq, a, c);
+    }
+
+    function AddPaths(p1: Path, p2: Path): (r: Path)
+        requires |p1.v| > 0
+        requires |p2.v| > 0
+        requires p1.v[|p1.v|-1] == p2.v[0]
+    {
+        var p2t := if |p2.v| > 1 then p2.v[1..|p2.v|] else [];
+        Path(p1.v + p2t)
+    }
+
+    lemma AddPathsValid(g: Digraph, p1: Path, p2: Path)
+        requires PathValid(g, p1)
+        requires PathValid(g, p2)
+        requires |p1.v| > 0
+        requires |p2.v| > 0
+        requires p1.v[|p1.v|-1] == p2.v[0]
+        ensures
+            var r := AddPaths(p1, p2);
+            PathValid(g, r)
+    {
+        reveal PathValid();
+    }
+    
+    lemma AddPathsFromTo(g: Digraph, p1: Path, p2: Path)
+        requires PathValid(g, p1)
+        requires PathValid(g, p2)
+        requires |p1.v| > 0
+        requires |p2.v| > 0
+        requires PathEnd(p1) == PathStart(p2)
+        ensures
+            var r := AddPaths(p1, p2);
+            var a := PathStart(p1);
+            var c := PathEnd(p2);
+            ShortPathFromTo(g, r, a, c) &&
+            |r.v| == |p1.v| + |p2.v| - 1
+    {
+        AddPathsValid(g, p1, p2);
+    }
+
+    // If there was already a path from b to a then adding a connection from a to b will
+    // create a loop.
+    lemma ConnectNodesDigraphLoop(g: Digraph, n: Node, m: Node)
+        requires g.IsNode(n) && g.IsNode(m) && n != m && !g.IsConnected(n, m)
+        //ensures
+        //    var r := ConnectNodes(g, n, m);
+        //    DigraphLoop(r) == DigraphLoop(g) || PathExists(g, m, n)
+    {
+        var r := ConnectNodes(g, n, m);
+        if DigraphLoop(g) {
+            reveal DigraphLoop();
+            var p: Path :| PathValid(g, p) && PathLoop(p);
+            ConnectNodesPathStillValid(g, n, m, p);
+            assert PathValid(r, p);
+            assert DigraphLoop(r);
+        }
+        ConnectNodesPathExists(g, n, m);
+        assert PathExists(r, n, m);
+        if PathExists(g, m, n) {
+            var p :| PathFromTo(g, p, m, n);
+            reveal PathValid();
+            assert PathFromTo(r, p, m, n);
+            ConnectNodesPathStillValid(g, n, m, p);
+            assert PathExists(r, m, n);
+            PathExistsAdd(r, n, m, n);
+            assert PathExists(r, n, n);
+            var q :| PathFromTo(r, q, n, n);
+            assert PathLoop(q);
+            reveal DigraphLoop();
+            assert DigraphLoop(r);
+        }
+        if DigraphLoop(r) {
+            reveal DigraphLoop();
+            if !DigraphLoop(g) {
+                var p :| PathValid(r, p) && PathLoop(p);
+                assert !PathValid(g, p);
+                reveal PathValid();
+                // First assume that n to m is not in the path.
+                // Then prove that this is not possible.
+                if !exists index: nat :: index < |p.v|-1 && (p.v[index] == n) && (p.v[index+1] == m) {
+                    forall index: nat | index < |p.v|-1
+                        ensures g.IsConnected(p.v[index], p.v[index+1]);
+                    {
+                        assert r.IsConnected(p.v[index], p.v[index+1]);
+                        assert g.IsConnected(p.v[index], p.v[index+1]);
+                    }
+                    assert false;
+                }
+                assert exists index: nat :: index < |p.v|-1 && (p.v[index] == n) && (p.v[index+1] == m);
+                var index: nat :| index < |p.v|-1 && (p.v[index] == n) && (p.v[index+1] == m);
+                assert PathStart(p) == PathEnd(p);
+                var q_1 := PathSegment(p, index+1, |p.v|);
+                assert |q_1.v| > 0;
+                assert PathEnd(q_1) == PathEnd(p);
+                PathSegmentValid(r, p, index+1, |p.v|);
+                assert PathValid(r, q_1);
+                var q_2 := PathSegment(p, 0, index+1);
+                assert PathStart(q_2) == PathStart(p);
+                assert PathStart(q_2) == PathEnd(q_1);
+                PathSegmentValid(r, p, 0, index+1);
+                var q := AddPaths(q_1, q_2);
+                AddPathsValid(r, q_1, q_2);
+                assert PathValid(r, q);
+                AddPathsFromTo(r, q_1, q_2);
+                assert PathFromTo(r, q, m, n);
+                // We want to now show that [n, m] does not appear in q.
+                // We actually need to find another path that removes any repeats and then
+                // show that that does not include [n, m]
+                // Then we can show that that is valid in g.
+                var s := PathRemoveLoops(q);
+                RemoveLoopsFromToSame(r, q);
+                assert PathFromTo(r, s, m, n);
+                assert PathValid(r, s);
+                assert PathNoRepeats(s);
+                forall index: nat | index < |s.v|-1 {
+                    var n1 := s.v[index];
+                    var n2 := s.v[index+1];
+                    //assert if index == 0 then n1 == m else n1 != m;
+                    assert r.IsConnected(s.v[index], s.v[index+1]);
+                    assert !((n1 == n) && (n2 == m));
+                    assert g.IsConnected(s.v[index], s.v[index+1]);
+                }
+                assert PathValid(g, s);
+                assert PathFromTo(g, s, m, n);
+            }
+            //assert DigraphLoop(g) || PathExists(g, m, n);
+        }
     }
 }
